$$\frac{d}{dx}(ax^{n}) = (a.n)x^{n-1}$$
- a is a constant,
- x is the variable,
- n is the exponent.

### Combinations
##### Derivative of a Constant
If f(x)=a (a constant), then:
$$\frac{d}{dx}(a) = 0$$
Reason: A constant does not change, so its rate of change is zero.

##### Derivative of x^n (No Coefficient)
If f(x)=x^n, the coefficient a=1, so:

$$\frac{d}{dx}(x^n) = n \cdot x^{n-1}$$

##### Combinations of Terms

When a function is the sum or difference of multiple terms, the derivative of the whole function is the **sum or difference of the derivatives** of its parts:

$$\frac{d}{dx}(f(x) + g(x)) = \frac{d}{dx}(f(x)) + \frac{d}{dx}(g(x))$$

Similarly:

$$\frac{d}{dx}(f(x) - g(x)) = \frac{d}{dx}(f(x)) - \frac{d}{dx}(g(x))$$

##### Negative exponent
$$y=\frac{3}{x^6}+\frac{2}{x^{-3}}$$
$$y=3x^{-6}+2x^{3}$$
Then apply the power rule.

[[Manipulating exponent]]

##### Square-root 

$$y=3\sqrt{x} - 2\sqrt[4]{x^6}$$
$$y=3x^{\frac{1}{2}} - 2(x^6)^{\frac{1}{4}}$$
$$y=3x^{\frac{1}{2}} - 2x^{\frac{3}{2}}$$
Then apply the power rule.

[[Manipulating exponent]]

##### Product of two functions
$$\frac{d}{dx}f(x)g(x)=f^{\prime}(x)g(x)+f(x)g^{\prime}(x)$$
$$y=ABC$$
$$y^{\prime}=A^{\prime}BC+AB^{\prime}C+ABC^{\prime}$$

Example:
$$h(x)=(\frac{1}{xÂ²}-\frac{3}{x^4})(x+5x^3)$$
$$h(x)=(x^{-2}-3x^{-4})(x+5x^3)$$
$$h^{\prime}(x)=(-2x^{-3}+12x^{-5})(x+5x^3) + (x^{-2}-3x^{-4})(1 +15x^2)$$


[[Calculate fractions]]